code/aes/Hacl.Impl.AES.SubBytes.fsti
@@ -6,6 +6,8 @@ module S = Lib.Sliceable
 
 open FStar.HyperStack.ST
 
+#set-options "--fuel 0 --ifuel 0"
+
 inline_for_extraction noextract
 let u64 = S.uN IT.U64 IT.SEC
 
@@ -13,10 +15,17 @@ inline_for_extraction noextract
 val sbox (s:nat{s<256}) : (r:nat{r<256})
 
 inline_for_extraction noextract
-val sub_bytes_spec (#n:IT.size_nat) (#xN:S.sig n) (x:S.xNxM xN 8) : S.xNxM xN 8
+val sbox_inv (s:nat{s<256}) : (r:nat{r<256})
 
-val sub_bytes_spec_theorem (#n:IT.size_nat) (#xN:S.sig n) (x:S.xNxM xN 8) (j:nat{j<n})
-  : Lemma ( S.column j (sub_bytes_spec x) == S.of_uint (sbox (S.to_uint (S.column j x))) )
+val sbox_inv_theorem (s:nat{s<256}) : Lemma (sbox_inv (sbox s) == s)
+
+// sub_bytes
+
+inline_for_extraction noextract
+val sub_bytes (#n:IT.size_nat) (#xN:S.sig n) (x:S.xNxM xN 8) : S.xNxM xN 8
+
+val sub_bytes_theorem (#n:IT.size_nat) (#xN:S.sig n) (x:S.xNxM xN 8) (j:nat{j<n})
+  : Lemma ( S.column j (sub_bytes x) == S.of_uint (sbox (S.to_uint (S.column j x))) )
 
 val sub_bytes64x8
   (st0:u64.t) (st1:u64.t) (st2:u64.t) (st3:u64.t)
@@ -27,5 +36,25 @@ val sub_bytes64x8
       (fun h0 (o0,o1,o2,o3,o4,o5,o6,o7) h1 ->
         B.modifies LowStar.Monotonic.Buffer.loc_none h0 h1
         /\ S.uNx8_mk o0 o1 o2 o3 o4 o5 o6 o7
-          == sub_bytes_spec (S.uNx8_mk st0 st1 st2 st3 st4 st5 st6 st7)
+          == sub_bytes (S.uNx8_mk st0 st1 st2 st3 st4 st5 st6 st7)
+      )
+
+// sub_bytes_inv
+
+inline_for_extraction noextract
+val sub_bytes_inv (#n:IT.size_nat) (#xN:S.sig n) (x:S.xNxM xN 8) : S.xNxM xN 8
+
+val sub_bytes_inv_theorem (#n:IT.size_nat) (#xN:S.sig n) (x:S.xNxM xN 8) (j:nat{j<n})
+  : Lemma ( S.column j (sub_bytes_inv x) == S.of_uint (sbox_inv (S.to_uint (S.column j x))) )
+
+val sub_bytes_inv64x8
+  (st0:u64.t) (st1:u64.t) (st2:u64.t) (st3:u64.t)
+  (st4:u64.t) (st5:u64.t) (st6:u64.t) (st7:u64.t) :
+    Stack
+      (u64.t * u64.t * u64.t * u64.t * u64.t * u64.t * u64.t * u64.t)
+      (fun _ -> True)
+      (fun h0 (o0,o1,o2,o3,o4,o5,o6,o7) h1 ->
+        B.modifies LowStar.Monotonic.Buffer.loc_none h0 h1
+        /\ S.uNx8_mk o0 o1 o2 o3 o4 o5 o6 o7
+          == sub_bytes_inv (S.uNx8_mk st0 st1 st2 st3 st4 st5 st6 st7)
       )
